Lean4Lean/Verify/TypeChecker/Basic.lean
@@ -192,7 +192,7 @@ structure VContext extends Context where
   hasPrimitives : VEnv.HasPrimitives venv
   safePrimitives : env.find? n = some ci →
     Environment.primitives.contains n → ci.safety = .safe ∧ ci.levelParams = []
-  trenv : TrEnv safety env venv
+  trenv : CheckingEnv safety env venv
   mlctx : MLCtx
   mlctx_wf : mlctx.WF venv lparams
   lctx_eq : mlctx.lctx = lctx
